src/usuba_sem.v
@@ -2,14 +2,18 @@ Require Import Coq.FSets.FMapPositive.
 Module PM := Coq.FSets.FMapPositive.PositiveMap.
 
 Require Import Coq.ZArith.ZArith.
+Require Import List.
+Import ListNotations.
 
 (*****************************************************************)
 
 (* XXX: lengthy prelude *)
 
-Axiom Zrotl: Z -> Z -> Z.
-Axiom Zrotr: Z -> Z -> Z.
-
+Definition fmap {A B} (f: A -> B)(x: option A) : option B :=
+  match x with
+  | None => None
+  | Some i => Some (f i)
+  end.
 
 Definition bind {A B} (x: option A)(f : A -> option B): option B :=
   match x with
@@ -24,11 +28,14 @@ Notation "'let!' x ':=' ma 'in' f" :=
 Notation "'ret!' x" := (Some x)
                          (at level 200).
 
+Notation "'fail!'" := (None)
+                         (at level 200).
+
 Inductive val := 
-| Base: bool -> val
+| Atom: bool -> val
 | Tup: list val -> val.
 
-Definition value := option val.
+Definition value := (*option*) val.
 Definition Env := PM.t value.
 
 (*****************************************************************)
@@ -36,7 +43,7 @@ Definition Env := PM.t value.
 Require Import usuba_AST.
 
 
-Definition sem_log_op (op: log_op) :=
+Definition sem_log_op (op: log_op): bool -> bool -> bool :=
   match op with
   | And => andb
   | Or => orb
@@ -44,7 +51,7 @@ Definition sem_log_op (op: log_op) :=
   | Andn => (fun x y => negb (andb x y))
   end.
 
-Definition sem_arith_op (op: arith_op) :=
+Definition sem_arith_op (op: arith_op): Z -> Z -> Z :=
    match op with
    | Add => Z.add
    | Mul => Z.mul
@@ -53,51 +60,111 @@ Definition sem_arith_op (op: arith_op) :=
    | Mod => Z.modulo
    end.
 
-Definition sem_shift_op (op: shift_op) := 
+(* XXX: shifts are a bit dodgy, they potentially introduce ill-typed data *)
+Definition sem_shift_op (op: shift_op): list val -> nat -> list val.
+refine (
   match op with
-  | Lshift => Z.shiftl
-  | Rshift => Z.shiftr
-  | Lrotate => Zrotl
-  | Rrotate => Zrotr
-  end.
+  | Lshift => _
+  | Rshift => _
+  | Lrotate => _
+  | Rrotate => _
+  end).
+Admitted.
 
 (* Arithmetic expressions, fully-reduced at compile-time *)
 Fixpoint sem_arith_expr (ae: arith_expr)(env: PM.t Z): option Z :=
   match ae with
   | Const_e i => Some i
-  | Var_e x => PM.find x env
+  | Var_e x => PM.find (uid x) env
   | Op_e op e1 e2 => let! x := sem_arith_expr e1 env in
                     let! y := sem_arith_expr e2 env in
                     Some (sem_arith_op op x y)
   end.
 
-Inductive sem_var (env: PM.t value): var -> value -> Prop :=.
+Print var.
 
-Inductive sem_expr (env: PM.t value): expr -> value -> Prop :=
+Definition val_lookup (v: val)(k: Z): option val :=
+  match v with
+  | Atom _ => None
+  | Tup xs => List.nth_error xs (Z.to_nat k)
+  end.
+
+Fixpoint mask {A}(l: list A)(k1 k2: nat): option (list A) :=
+  match k2 with
+  | 0 => ret! []
+  | S k2 => 
+    match k1 with
+    | S k1 => match l with
+             | [] => fail!
+             | x :: xs => mask xs k1 k2
+             end
+    | 0 => match l with
+          | [] => fail!
+          | x :: xs => 
+            let! xs := mask xs 0 k2 in
+            ret! (x :: xs)
+          end
+    end
+  end.
+
+Lemma test__mask: mask [0; 1; 2; 3; 4; 5; 6; 7] 2 5 = Some [2; 3; 4].
+Proof. auto. Qed.
+
+Definition val_mask (v: val)(k1 k2: Z): option val :=
+  match v with
+  | Atom _ => None
+  | Tup xs => fmap Tup (mask xs (Z.to_nat k1) (Z.to_nat k2))
+  end.
+
+Section SemExpr.
+
+Variable prog: PM.t def.
+Variable senv: PM.t Z.
+
+Inductive sem_var (env: PM.t value): var -> value -> Prop :=
+| sem_Var: forall x v,
+    PM.find (uid x) env = Some v ->
+    sem_var env (Var x) v
+| sem_Slice: forall x aes ks vx vs,
+    sem_var env x vx ->
+    Forall2 (fun ae k => sem_arith_expr ae senv = Some k) aes ks ->
+    Forall2 (fun k v => val_lookup vx k = Some v) ks vs ->
+    sem_var env (Slice x aes) (Tup vs)
+| sem_Range: forall x ae1 ae2 k1 k2 vx v,
+    sem_var env x vx ->
+    sem_arith_expr ae1 senv = Some k1 ->
+    sem_arith_expr ae2 senv = Some k2 ->
+    val_mask vx k1 k2 = Some v ->
+    sem_var env (Range x ae1 ae2) v.
+
+Inductive sem_expr: PM.t value -> expr -> value -> Prop :=
 (* XXX: problem with const: to which tuple do we compile to? *)
 (*| sem_Const: forall i,
     sem_expr (Const i) (Some ?).
 *)
-| sem_ExpVar: forall v i,
+| sem_ExpVar: forall env v i,
     sem_var env v i ->
     sem_expr env (ExpVar v) i
-| sem_Tuple: forall es vs,
-    (* XXX: need a suitable definition, taking care of absences *)
-    List.Forall2 (sem_expr env) es (List.map Some vs) ->
-    sem_expr env (Tuple es) (Some (Tup vs))
-(*
-| sem_Not: forall e b v,
-    sem_expr env e (Base b) ->
-    sem_expr env (Not e) (Base (negb b)). (* special case for bitwise not *)
-  | Shift (op: shift_op)(e: expr)(ae: arith_expr)
-  | Log  (op: log_op)(e1 e2: expr)
-  | Arith (op: arith_op)(e1 e2: expr)
-  | Intr (i: intr_fun)(e1 e2: expr)
-  | Fun (x: ident)(es: list expr)
-  | Fun_v (x: ident)(ae: arith_expr)(es: list expr) (* nodes arrays *)
-  | Fby (e1 e2: expr)(mx: option ident)
-  | When (e: expr)(x: constr) (y: ident)
-  | Merge (x: ident)(xs: list (constr * expr))
-  | Nop.
-
-*)
+| sem_Tuple: forall env es vs,
+    List.Forall2 (sem_expr env) es vs ->
+    sem_expr env (Tuple es) (Tup vs)
+| sem_Not: forall env e b,
+    sem_expr env e (Atom b) ->
+    sem_expr env (Not e) (Atom (negb b))
+| sem_Shift: forall env op e ae k ve v,
+    sem_expr env e (Tup ve) ->
+    sem_arith_expr ae senv = Some k ->
+    sem_shift_op op ve (Z.to_nat k) = v ->
+    sem_expr env (Shift op e ae) (Tup v)
+| sem_Log: forall env op e1 e2 b1 b2 v,
+    sem_expr env e1 (Atom b1) ->
+    sem_expr env e2 (Atom b2) ->
+    sem_log_op op b1 b2 = v ->
+    sem_expr env (Log op e1 e2) (Atom v)
+| sem_Fun: forall env f es node vs v,
+    PM.find (uid f) prog = Some node ->
+    Forall2 (sem_expr env) es vs ->
+    sem_node node vs v ->
+    sem_expr env (Fun f es) v
+with sem_node: def -> list value -> value -> Prop :=
+ (* XXX: stopped here *).
